Phi_System/IDE_CP_Reasoning2.thy
@@ -101,35 +101,6 @@ lemma [\<phi>reason 1000]:
   unfolding Remove_Values_def
   by simp 
 
-subsection \<open>Extract Elimination Rule\<close>
-
-definition Extract_Elimination_Rule :: \<open>prop \<Rightarrow> bool \<Rightarrow> bool \<Rightarrow> prop\<close>
-  where \<open>Extract_Elimination_Rule IN OUT_L OUT_R \<equiv> (PROP IN \<Longrightarrow> OUT_L \<Longrightarrow> OUT_R)\<close>
-
-declare [[\<phi>reason_default_pattern \<open>PROP Extract_Elimination_Rule ?I ?L ?R\<close>
-                                \<Rightarrow> \<open>PROP Extract_Elimination_Rule ?I ?L ?R\<close> (100) ]]
-
-lemma Do_Extract_Elimination_Rule:
-  \<open> PROP IN
-\<Longrightarrow> PROP Extract_Elimination_Rule IN OUT_L OUT_R
-\<Longrightarrow> OUT_L \<Longrightarrow> (OUT_R \<Longrightarrow> C) \<Longrightarrow> C\<close>
-  unfolding Extract_Elimination_Rule_def
-proof -
-  assume IN: \<open>PROP IN\<close>
-    and  RL: \<open>PROP IN \<Longrightarrow> OUT_L \<Longrightarrow> OUT_R\<close>
-    and  OL: \<open>OUT_L\<close>
-    and  OR: \<open>OUT_R \<Longrightarrow> C\<close>
-  from OR[OF RL[OF IN OL]] show \<open>C\<close> .
-qed
-
-lemma [\<phi>reason 1100]:
-  \<open>PROP Extract_Elimination_Rule (Trueprop (X \<^bold>i\<^bold>m\<^bold>p\<^bold>l\<^bold>i\<^bold>e\<^bold>s Y)) (Inhabited X) (Inhabited Y) \<close>
-  unfolding Extract_Elimination_Rule_def Imply_def Inhabited_def by blast
-
-lemma [\<phi>reason 1000]:
-  \<open>PROP Extract_Elimination_Rule (Trueprop (X \<^bold>i\<^bold>m\<^bold>p\<^bold>l\<^bold>i\<^bold>e\<^bold>s Y \<^bold>a\<^bold>n\<^bold>d P)) (Inhabited X) (Inhabited Y \<and> P) \<close>
-  unfolding Extract_Elimination_Rule_def Imply_def Inhabited_def by blast
-
 
 subsection \<open>Rewrite into \<phi>-Type\<close>
 
